implemented twolockmsq in Iris. Created boilerplate for specs. Getting weird errors.

iris/twoLockMSQ.v
@@ -1,8 +1,0 @@
-From iris.heap_lang Require Import lang proofmode notation.
-
-Context `{!heapGS Σ}.
-
-(* TODO: implement *)
-Definition initialize : expr := #().
-Definition enqueue : expr := #().
-Definition dequeue : expr := #().
