theories/twoLockMSQ.v
@@ -1,0 +1,63 @@
+From iris.heap_lang Require Import lang proofmode notation.
+From iris.heap_lang.lib Require Import lock spin_lock.
+
+Definition initialize `{!lock} : val := 
+	rec: "initialize" <> := 
+		let: "node" := ref (SOME (NONE, ref(NONE))) in
+		let: "H_lock" := newlock #() in
+		let: "T_lock" := newlock #() in
+		ref (("node", "node"), ("H_lock", "T_lock")).
+
+Definition enqueue `{!lock} : val := 
+	rec: "enqueue" "Q" "value" :=
+		let: "node" := ref (SOME (SOME "value", ref(NONE))) in
+		acquire (Snd ( Snd (!"Q")));; (* Acqurie T_lock*)
+		let: "old_tail" := 
+			SOME (Fst ("get_some" (!(Snd (Fst(!"Q"))))), "node") in
+		(Snd (Fst!"Q")) <- "old_tail" ;;
+		"Q" <- ((Fst (Fst (!"Q")), "node"), Snd(!"Q")) ;;
+		release (Snd (Snd (!"Q"))).
+
+Definition dequeue `{!lock}: val := 
+	rec: "dequeue" "Q" := 
+		acquire (Fst (Snd (!"Q")));; (* Acquire H_lock*)
+		let: "node" := (Fst (Fst (!"Q"))) in
+		let: "new_head" := Snd("get_some" (!"node")) in
+		if: "new_head" = NONEV then
+			release (Fst (Snd(!"Q"))) ;;
+			NONEV
+		else
+			let: "value" := (Fst (!"new_head")) in
+			"Q" <- (("new_head", (Snd(Fst(!"Q")))), Snd (! "Q"));;
+			release (Fst (Snd (!"Q")));;
+			"value".
+
+
+Section proofs.
+
+Context `{!heapGS Σ}.
+Context `{!lockG Σ}.
+Let N := nroot .@ "twoLockMSQ".
+
+(* Definition queue_invariant (head tail : loc) : iProp Σ := 
+	∃ xs, isList xs . *)
+
+Definition is_queue (v : val) : iProp Σ := 
+	∃ head tail : loc, ∃ H_lock T_lock : val, ∃ γH γT : gname, 
+	∃ l : loc , ⌜v = #l⌝ ∗ l ↦ ((#head, #tail), (H_lock, T_lock))
+	∗ True (* H_lock is a lock*)
+	∗ True. (* T_lock is a lock*)
+
+Lemma initialize_spec : {{{ True }}} initialize #() {{{v, RET v; True}}}.
+Proof.
+	Admitted.
+
+Lemma enqueue_spec Q v : {{{ True }}} enqueue Q #v {{{v, RET v; True}}}.
+Proof.
+	Admitted.
+
+Lemma dequeue_spec Q : {{{ True }}} dequeue Q {{{v, RET v; True}}}.
+Proof.
+	Admitted.
+
+End proofs.
